src/lib/invariants.v
@@ -1,0 +1,307 @@
+From stdpp Require Export namespaces.
+From iris.algebra Require Import gmap.
+From iris.proofmode Require Import proofmode.
+From nextgen.lib Require Import wsat.
+From nextgen.lib Require Export fancy_updates.
+From nextgen Require Import nextgen_pointwise.
+From iris.prelude Require Import options.
+Import uPred.
+Import le_upd_if.
+
+
+(** In the base logic of Iris, invariants are defined semantically,
+    while the internal model of invariants is abstracted away.
+
+    In this version, we expose the true definition of invariants, to
+    allow for easy proof of a nextgen introduction.  Alternatively,
+    one needs to express the introduction of a transformation into Ω
+*)
+
+(** ** Semantic definition of invariants (do not survive a nextgen) *)
+Local Definition inv_def `{!invGIndS_gen hlc Σ Ω A pick} (N : namespace) (c : C) (P : iProp Σ) : iProp Σ :=
+  □ ∀ E, ⌜↑N ⊆ E⌝ → (* ∀ c', ⌜CR c c'⌝ →  *)
+    (* ⚡={transmap_insert_two_inG (inv_pick_transform c') (C_pick c') Ω}=> *)
+    |={E,E ∖ ↑N}=> ▷ P ∗ (▷ P ={E ∖ ↑N,E}=∗ True).
+Local Definition inv_aux : seal (@inv_def). Proof. by eexists. Qed.
+Definition inv_sem := inv_aux.(unseal).
+Global Arguments inv_sem {hlc Σ Ω A pick _} N c P.
+Local Definition inv_sem_unseal : @inv_sem = @inv_def := inv_aux.(seal_eq).
+Global Instance: Params (@inv_sem) 4 := {}.
+
+(** ** Internal model of invariants *)
+Local Definition own_inv `{!invGIndS_gen hlc Σ Ω A pick} (N : namespace) (c : C) (P : iProp Σ) : iProp Σ :=
+  ∃ i, ⌜i ∈ (↑N:coPset)⌝ ∧ ownI i P ∧ ownC i c.
+Local Definition own_inv_aux : seal (@own_inv). Proof. by eexists. Qed.
+Definition inv := own_inv_aux.(unseal).
+Global Arguments inv {hlc Σ Ω A pick _} N c P.
+Local Definition inv_unseal : @inv = @own_inv := own_inv_aux.(seal_eq).
+Global Instance: Params (@inv) 4 := {}.
+
+(** * Invariants *)
+Section inv.
+  Context `{!invGIndS_gen hlc Σ Ω A pick}.
+  Implicit Types i : positive.
+  Implicit Types N : namespace.
+  Implicit Types E : coPset.
+  Implicit Types P Q R : iProp Σ.
+
+  Lemma own_inv_acc E N c P :
+    ↑N ⊆ E → own_inv N c P ⊢
+          |={E,E∖↑N}=> ▷ P ∗ (▷ P ={E∖↑N,E}=∗ True).
+  Proof.
+    rewrite fancy_updates.uPred_fupd_unseal /fancy_updates.uPred_fupd_def.
+    iDestruct 1 as (i) "[Hi #[HiP HiC]]".
+    iDestruct "Hi" as % ?%elem_of_subseteq_singleton.
+    (* iIntros (c' HCR). *)
+    (* iDestruct (frag_invariant_insert_intro (inv_pick_transform c') with "HiP") as "HiP'". *)
+    (* iDestruct (frag_pick_map_transform_Some_intro with "HiC") as "HiC'";[eauto|]. iClear "HiP HiC". *)
+    (* iModIntro. *)
+    (* iDestruct (frag_invariant_insert_intro (C_pick c') with "HiP'") as "HiP". *)
+    (* iDestruct (frag_pick_map_insert_intro _ _ (C_pick c') with "HiC'") as "HiC". iClear "HiP' HiC'". *)
+    (* iModIntro. *)
+    rewrite {1 4}(union_difference_L (↑ N) E) // wsat.ownE_op; last set_solver.
+    rewrite {1 5}(union_difference_L {[ i ]} (↑ N)) // wsat.ownE_op; last set_solver.
+    iIntros "(Hw & [HE $] & $) !> !>".
+    iDestruct (ownI_open i with "[$Hw $HE $HiP $HiC]") as "($ & $ & HD)".
+    iIntros "HP [Hw $] !> !>". iApply (ownI_close _ c P). by iFrame "∗ #".
+  Qed.
+
+  Lemma fresh_inv_name (E : gset positive) N : ∃ i, i ∉ E ∧ i ∈ (↑N:coPset).
+  Proof.
+    exists (coPpick (↑ N ∖ gset_to_coPset E)).
+    rewrite -elem_of_gset_to_coPset (comm and) -elem_of_difference.
+    apply coPpick_elem_of=> Hfin.
+    eapply nclose_infinite, (difference_finite_inv _ _), Hfin.
+    apply gset_to_coPset_finite.
+  Qed.
+
+  Lemma own_inv_alloc N E c P : inv_cond P c ∗ ▷ P ={E}=∗ own_inv N c P.
+  Proof.
+    rewrite fancy_updates.uPred_fupd_unseal /fancy_updates.uPred_fupd_def.
+    iIntros "[#Hcond HP] [Hw $]".
+    iMod (ownI_alloc (.∈ (↑N : coPset)) P with "[$HP $Hw $Hcond]")
+      as (i ?) "[$ [? ?]]"; auto using fresh_inv_name.
+    do 2 iModIntro. iExists i. auto.
+  Qed.
+
+  (* This does not imply [own_inv_alloc] due to the extra assumption [↑N ⊆ E]. *)
+  Lemma own_inv_alloc_open N E c P :
+    ↑N ⊆ E → inv_cond P c ⊢ |={E, E∖↑N}=> own_inv N c P ∗ (▷ P ={E∖↑N, E}=∗ True).
+  Proof.
+    iIntros (Sub) "#Hcond".
+    rewrite fancy_updates.uPred_fupd_unseal /fancy_updates.uPred_fupd_def.
+    iIntros "[Hw HE]".
+    iMod (ownI_alloc_open (.∈ (↑N : coPset)) P with "[$Hcond $Hw]")
+      as (i ?) "(Hw & #Hi & #Hc & HD)"; auto using fresh_inv_name.
+    iAssert (ownE {[i]} ∗ ownE (↑ N ∖ {[i]}) ∗ ownE (E ∖ ↑ N))%I
+      with "[HE]" as "(HEi & HEN\i & HE\N)".
+    { rewrite -?wsat.ownE_op; [|set_solver..].
+      rewrite assoc_L -!union_difference_L //. set_solver. }
+    do 2 iModIntro. iFrame "HE\N". iSplitL "Hw HEi"; first by iApply "Hw".
+    iSplitL "Hi".
+    { iExists i. auto. }
+    iIntros "HP [Hw HE\N]".
+    iDestruct (ownI_close with "[$Hw $Hi $Hc $HP $HD]") as "[$ HEi]".
+    do 2 iModIntro. iSplitL; [|done].
+    iCombine "HEi HEN\i HE\N" as "HEN".
+    rewrite -?wsat.ownE_op; [|set_solver..].
+    rewrite assoc_L -!union_difference_L //; set_solver.
+  Qed.
+
+  Lemma own_inv_to_inv M c P : own_inv M c P -∗ inv M c P.
+  Proof.
+    iIntros "#I". rewrite inv_unseal. auto.
+  Qed.
+
+  Lemma own_inv_to_sem_inv M c P : own_inv M c P -∗ inv_sem M c P.
+  Proof.
+    iIntros "#I". rewrite inv_sem_unseal.
+    iIntros (E H). iPoseProof (own_inv_acc with "I") as "H";[eauto|].
+    auto.
+  Qed.
+
+  Lemma inv_to_sem_inv M c P : inv M c P -∗ inv_sem M c P.
+  Proof.
+    rewrite inv_unseal.
+    iIntros "Hown".
+    iDestruct (own_inv_to_sem_inv with "Hown") as "$".
+  Qed.
+
+  (** ** Public API of invariants *)
+  Global Instance inv_contractive N c : Contractive (inv N c).
+  Proof.
+    rewrite inv_unseal.
+    rewrite /own_inv /=. intros ??? Hdist.
+    solve_contractive.
+  Qed.
+
+  Global Instance inv_ne N c : NonExpansive (inv N c).
+  Proof. apply contractive_ne, _. Qed.
+
+  Global Instance inv_proper N c : Proper (equiv ==> equiv) (inv N c).
+  Proof. apply ne_proper, _. Qed.
+
+  Global Instance inv_persistent N c P : Persistent (inv N c P).
+  Proof. rewrite inv_unseal. apply _. Qed.
+
+  Global Instance inv_sem_contractive N c : Contractive (inv_sem N c).
+  Proof.
+    rewrite inv_sem_unseal.
+    rewrite /inv_def /=. intros ??? Hdist.
+    solve_contractive.
+  Qed.
+
+  Global Instance inv_sem_ne N c : NonExpansive (inv_sem N c).
+  Proof. apply contractive_ne, _. Qed.
+
+  Global Instance inv_sem_proper N c : Proper (equiv ==> equiv) (inv_sem N c).
+  Proof. apply ne_proper, _. Qed.
+
+  Global Instance inv_sem_persistent N c P : Persistent (inv_sem N c P).
+  Proof. rewrite inv_sem_unseal. apply _. Qed.
+
+  Lemma inv_mod_intro N c P c' :
+    CR c c' ->
+    inv N c P ⊢ ⚡={transmap_insert_two_inG (inv_pick_transform c') (C_pick c') Ω}=> inv N c P.
+  Proof.
+    rewrite inv_unseal /own_inv.
+    iIntros (HCR) "#HI".
+    iDestruct "HI" as (i Hin) "[HI HC]".
+    iDestruct (frag_invariant_insert_two_intro with "HI") as "HI'".
+    iDestruct (frag_pick_map_transform_two_Some_intro with "HC") as "HC'";[eauto|].
+    iClear "HI HC". iModIntro. iExists _. iFrame "# %".
+  Qed.
+  
+  Lemma inv_alter N c P Q : inv_sem N c P -∗ ▷ □ (P -∗ Q ∗ (Q -∗ P)) -∗ inv_sem N c Q.
+  Proof.
+    rewrite inv_sem_unseal. iIntros "#HI #HPQ !>" (E H).
+    iMod ("HI" $! E H) as "[HP Hclose]".
+    iDestruct ("HPQ" with "HP") as "[$ HQP]".
+    iIntros "!> HQ". iApply "Hclose". iApply "HQP". done.
+  Qed.
+
+  Lemma inv_iff N c P Q : inv_sem N c P -∗ ▷ □ (P ↔ Q) -∗ inv_sem N c Q.
+  Proof.
+    iIntros "#HI #HPQ". iApply (inv_alter with "HI").
+    iClear "HI". iIntros "!> !> HP". iSplitL "HP".
+    - by iApply "HPQ".
+    - iIntros "HQ". by iApply "HPQ".
+  Qed.
+
+  Lemma inv_alloc N E c P : inv_cond P c ∗ ▷ P ={E}=∗ inv N c P.
+  Proof.
+    iIntros "[#Hcond HP]". iApply (own_inv_to_inv _ c).
+    iApply (own_inv_alloc N E with "[$HP $Hcond]").
+  Qed.
+
+  Lemma inv_alloc_open N E c P :
+    ↑N ⊆ E → inv_cond P c ⊢ |={E, E∖↑N}=> inv N c P ∗ (▷P ={E∖↑N, E}=∗ True).
+  Proof.
+    iIntros (?) "#Hcond".
+    iMod (own_inv_alloc_open with "[$]") as "[HI $]"; first done.
+    iApply own_inv_to_inv. done.
+  Qed.
+
+  Lemma inv_acc E N c P :
+    ↑N ⊆ E → ⊢ inv N c P →
+          |={E,E∖↑N}=> ▷ P ∗ (▷ P ={E∖↑N,E}=∗ True).
+  Proof.
+    iIntros (?) "#HI".
+    iDestruct (inv_to_sem_inv with "HI") as "HI'".
+    rewrite inv_sem_unseal /inv_def.
+    by iApply "HI'".
+  Qed.
+
+  Lemma inv_combine N1 N2 N c P Q :
+    N1 ## N2 →
+    ↑N1 ∪ ↑N2 ⊆@{coPset} ↑N →
+    inv_sem N1 c P -∗ inv_sem N2 c Q -∗ inv_sem N c (P ∗ Q).
+  Proof.
+    rewrite inv_sem_unseal. iIntros (??) "#HinvP #HinvQ !>"; iIntros (E ?).
+    iMod ("HinvP" $! E with "[%]") as "[$ HcloseQ]";[set_solver|].
+    iMod ("HinvQ" $! (E ∖ ↑N1) with "[%]") as "[$ HcloseP]";[set_solver|].
+    iApply fupd_mask_intro; first set_solver.
+    iIntros "Hclose [HP HQ]".
+    iMod "Hclose" as %_. iMod ("HcloseP" with "HQ") as %_.
+    by iApply "HcloseQ".
+  Qed.
+
+  Lemma inv_combine_dup_l N c P Q :
+    □ (P -∗ P ∗ P) -∗
+    inv_sem N c P -∗ inv_sem N c Q -∗ inv_sem N c (P ∗ Q).
+  Proof.
+    rewrite inv_sem_unseal. iIntros "#HPdup #HinvP #HinvQ !>" (E ?).
+    iMod ("HinvP" with "[//]") as "[HP HcloseP]".
+    iDestruct ("HinvQ" with "[//]") as "HQ". 
+    iDestruct ("HPdup" with "HP") as "[$ HP]".
+    iMod ("HcloseP" with "HP") as %_.
+    iMod "HQ" as "[$ HcloseQ]".
+    iIntros "!> [HP HQ]". by iApply "HcloseQ".
+  Qed.
+
+  Lemma except_0_inv N c P : ◇ inv_sem N c P ⊢ inv_sem N c P.
+  Proof.
+    rewrite inv_sem_unseal /inv_def. iIntros "#H !>" (E HE).
+    iSpecialize ("H" $! E HE).
+    iMod "H". by iApply "H".
+  Qed.
+
+  (** ** Proof mode integration *)
+  Global Instance is_except_0_inv N c P : IsExcept0 (inv_sem N c P).
+  Proof. apply except_0_inv. Qed.
+
+  Global Instance into_inv_inv N c P : IntoInv (inv N c P) N := {}.
+  Global Instance into_inv_sem_inv N c P : IntoInv (inv_sem N c P) N := {}.
+
+  Global Instance into_acc_inv N c P E:
+    IntoAcc (X := unit) (inv N c P)
+            (↑N ⊆ E) True (fupd E (E ∖ ↑N)) (fupd (E ∖ ↑N) E)
+            (λ _ : (), (▷ P)%I) (λ _ : (), (▷ P)%I) (λ _ : (), None).
+  Proof.
+    rewrite /IntoAcc /accessor bi.exist_unit.
+    iIntros (?) "#Hinv _".
+    iApply inv_acc;eauto.
+  Qed.
+
+  (** ** Derived properties *)
+  Lemma inv_acc_strong E N c P :
+    ↑N ⊆ E → ⊢ inv N c P →
+          |={E,E∖↑N}=> ▷ P ∗ ∀ E', ▷ P ={E',↑N ∪ E'}=∗ True.
+  Proof.
+    iIntros (?) "Hinv".
+    iPoseProof (inv_acc (↑ N) N with "Hinv") as "H"; first done.
+    rewrite difference_diag_L.
+    iPoseProof (fupd_mask_frame_r _ _ (E ∖ ↑ N) with "H") as "H"; first set_solver.
+    rewrite left_id_L -union_difference_L //. iMod "H" as "[$ H]"; iModIntro.
+    iIntros (E') "HP".
+    iPoseProof (fupd_mask_frame_r _ _ E' with "(H HP)") as "H"; first set_solver.
+    by rewrite left_id_L.
+  Qed.
+
+  Lemma inv_acc_timeless E N c P `{!Timeless P} :
+    ↑N ⊆ E → ⊢ inv N c P →
+    |={E,E∖↑N}=> P ∗ (P ={E∖↑N,E}=∗ True).
+  Proof.
+    iIntros (?) "Hinv".
+    iDestruct (inv_acc with "Hinv") as "H";[eauto|].
+    iMod "H" as "[>HP Hclose]"; auto.
+    iIntros "!> {$HP} HP". iApply "Hclose"; auto.
+  Qed.
+
+  Lemma inv_split_l N c P Q : inv_sem N c (P ∗ Q) -∗ inv_sem N c P.
+  Proof.
+    iIntros "#HI". iApply inv_alter; eauto.
+    iClear "HI". iIntros "!> !> [$ $] $".
+  Qed.
+  Lemma inv_split_r N c P Q : inv_sem N c (P ∗ Q) -∗ inv_sem N c Q.
+  Proof.
+    rewrite (comm _ P Q). eapply inv_split_l.
+  Qed.
+  Lemma inv_split N c P Q : inv_sem N c (P ∗ Q) -∗ inv_sem N c P ∗ inv_sem N c Q.
+  Proof.
+    iIntros "#H".
+    iPoseProof (inv_split_l with "H") as "$".
+    iPoseProof (inv_split_r with "H") as "$".
+  Qed.
+
+End inv.
